theories/rust_typing/automation/loc_eq.v
@@ -107,7 +107,7 @@ Section test.
   solve_loc_eq. Qed.
 
   Goal (l offsetst{IntSynType u8}ₗ n1) = l +ₗ (ly_size u8 * n1).
-  init_cache; solve_loc_eq. Qed.
+  init_cache. solve_loc_eq. Qed.
 
   Goal (l offsetst{IntSynType usize_t}ₗ n1) = l +ₗ (ly_size usize_t * n1).
   init_cache; solve_loc_eq. Qed.
