theories/rust_typing/products.v
@@ -3787,8 +3787,70 @@ Section rules.
 
   (* TODO prove_place_cond *)
 
-  (* TODO resolve hgost *)
+  (** resolve_ghost instances *)
+  Lemma resolve_ghost_struct_Owned {rts} π E L l (lts : hlist ltype rts) sls γ wl rm lb T :
+    find_observation ((plist place_rfn rts)) γ FindObsModeDirect (λ or,
+        match or with
+        | None => ⌜rm = ResolveTry⌝ ∗ T L (PlaceGhost γ) True false
+        | Some r => T L (PlaceIn $ r) True true
+        end)
+    ⊢ resolve_ghost π E L rm lb l (StructLtype lts sls) (Owned wl) (PlaceGhost γ) T.
+  Proof.
+    iIntros "Ha" (???) "#CTX #HE HL Hl".
+    iMod ("Ha" with "[//]") as "[(%r' & HObs & Ha) | (_ & Ha)]".
+    - rewrite ltype_own_struct_unfold /struct_ltype_own.
+      iDestruct "Hl" as "(%sl & ? & ? & ? & ? & ? & %rs & Hinterp & ?)".
+      simpl. iPoseProof (gvar_pobs_agree_2 with "Hinterp HObs") as "#<-".
+      iExists _, _, _, _. iFrame. iApply maybe_logical_step_intro.
+      iL. rewrite ltype_own_struct_unfold /struct_ltype_own.
+      iExists _. iFrame. iExists _. iR. by iFrame.
+    - iExists _, _, _, _. iFrame.  iApply maybe_logical_step_intro. by iFrame.
+  Qed.
+  Definition resolve_ghost_struct_Owned_inst := [instance @resolve_ghost_struct_Owned].
+  Global Existing Instance resolve_ghost_struct_Owned_inst.
 
+  Lemma resolve_ghost_struct_Uniq {rts} π E L l (lts : hlist ltype rts) sls γ rm lb κ γ' T :
+    find_observation ((plist place_rfn rts)) γ FindObsModeDirect (λ or,
+        match or with
+        | None => ⌜rm = ResolveTry⌝ ∗ T L (PlaceGhost γ) True false
+        | Some r => T L (PlaceIn $ r) True true
+        end)
+    ⊢ resolve_ghost π E L rm lb l (StructLtype lts sls) (Uniq κ γ') (PlaceGhost γ) T.
+  Proof.
+    iIntros "Ha" (???) "#CTX #HE HL Hl".
+    iMod ("Ha" with "[//]") as "[(%r' & HObs & Ha) | (_ & Ha)]".
+    - rewrite ltype_own_struct_unfold /struct_ltype_own.
+      iDestruct "Hl" as "(%ly & ? & ? & ? & ? & ? & Hinterp & ?)".
+      simpl.
+      iPoseProof (Rel2_use_pobs with "HObs Hinterp") as "(%r2 & Hobs & ->)".
+      iExists _, _, _, _. iFrame. iApply maybe_logical_step_intro.
+      iL. rewrite ltype_own_struct_unfold /struct_ltype_own.
+      iExists _. iFrame. done.
+    - iExists _, _, _, _. iFrame.  iApply maybe_logical_step_intro. by iFrame.
+  Qed.
+  Definition resolve_ghost_struct_Uniq_inst := [instance @resolve_ghost_struct_Uniq].
+  Global Existing Instance resolve_ghost_struct_Uniq_inst.
+
+  Lemma resolve_ghost_struct_Shared {rts} π E L l (lts : hlist ltype rts) sls γ rm lb κ T :
+    find_observation (plist place_rfn rts) γ FindObsModeDirect (λ or,
+        match or with
+        | None => ⌜rm = ResolveTry⌝ ∗ T L (PlaceGhost γ) True false
+        | Some r => T L (#r) True true
+        end)
+    ⊢ resolve_ghost π E L rm lb l (StructLtype lts sls) (Shared κ) (PlaceGhost γ) T.
+  Proof.
+    iIntros "Ha" (???) "#CTX #HE HL Hl".
+    iMod ("Ha" with "[//]") as "[(%r' & HObs & Ha) | (_ & Ha)]".
+    - rewrite ltype_own_struct_unfold /struct_ltype_own.
+      iDestruct "Hl" as "(%sl & ? & ? & ? & ? & %rs & Hinterp & ?)".
+      simpl. iPoseProof (gvar_pobs_agree_2 with "Hinterp HObs") as "#<-".
+      iExists _, _, _, _. iFrame. iApply maybe_logical_step_intro.
+      iL. rewrite ltype_own_struct_unfold /struct_ltype_own.
+      iExists _. iFrame. iExists _. iR. by iFrame.
+    - iExists _, _, _, _. iFrame. iApply maybe_logical_step_intro. by iFrame.
+  Qed.
+  Definition resolve_ghost_struct_Shared_inst := [instance @resolve_ghost_struct_Shared].
+  Global Existing Instance resolve_ghost_struct_Shared_inst.
 End rules.
 
 Global Typeclasses Opaque MutEqltypeStructHFR.
