theories/rust_typing/shims.v
@@ -130,8 +130,10 @@ Lemma mem_align_of_typed `{RRGS : !refinedrustGS Σ} π T_rt T_st T_ly :
   ⊢ typed_function π (mem_align_of T_st) [] (<tag_type> type_of_mem_align_of T_rt T_st).
 Proof.
   start_function "mem_align_of" ( () ) ( [T_ty []] ) ( () ).
-  repeat liRStep. Unshelve.
+  repeat liRStep; liShow.
+  Unshelve.
   all: unshelve_sidecond.
+  simplify_layout_goal.
   by apply ly_align_in_usize.
 Qed.
 
@@ -279,7 +281,7 @@ Proof.
   iApply (typed_goto_acc _ _ _ _ _ loop_inv).
   { unfold_code_marker_and_compute_map_lookup. }
   liRStep; liShow. iExists 0%nat.
-  repeat liRStep. liShow.
+  repeat liRStep; liShow.
   iRename select (loop_inv _ _) into "Hinv".
   iDestruct "Hinv" as "(%i & -> & -> & Hcredit & Hlen & Hcount & Hsrc & Hdst & Hs & Ht)".
   repeat liRStep; liShow.
